ErasedList.v
@@ -1,0 +1,39 @@
+Require Export SystemFR.TypeSugar2.
+Require Export SystemFR.ErasedRecGen.
+Require Export SystemFR.ErasedSum.
+Require Export SystemFR.ErasedPair.
+Require Export SystemFR.ErasedTop.
+
+Opaque strictly_positive.
+
+Lemma open_reducible_nil:
+  forall tvars gamma,
+    [ tvars; gamma ⊨ tnil : List ].
+Proof.
+  intros.
+
+  apply open_reducible_fold_gen2 with 0;
+    repeat step || simp_spos;
+    eauto with sets.
+
+  apply open_reducible_left.
+  apply open_reducible_unit.
+Qed.
+
+Lemma open_reducible_cons:
+  forall tvars gamma h t T,
+    [ tvars; gamma ⊨ t : List ] ->
+    [ tvars; gamma ⊨ h : T ] ->
+    [ tvars; gamma ⊨ tcons h t : List ].
+Proof.
+  intros.
+
+  apply open_reducible_fold_gen2 with 0;
+    repeat step || simp_spos;
+    eauto with sets.
+
+  apply open_reducible_right.
+  apply open_reducible_pp;
+    repeat step; eauto with sets;
+    eauto using open_reducible_top.
+Qed.
