ErasedSubtypeList.v
@@ -1,0 +1,14 @@
+Require Export SystemFR.ErasedList.
+
+Opaque reducible_values.
+Opaque Nil.
+Opaque List.
+
+Lemma nil_subtype_list:
+  forall tvars gamma,
+    [ tvars; gamma ⊨ Nil <: List ].
+Proof.
+  unfold subtype;
+    repeat step.
+
+    
