TypeSugar2.v
@@ -1,0 +1,27 @@
+Require Export SystemFR.ShiftOpen.
+
+Definition tsingleton t :=
+  T_type_refine T_top (T_equiv (lvar 0 term_var) (shift 0 t 1)).
+
+Definition type_application T1 T2 : tree :=
+  T_type_refine T_top (
+    T_exists T1 (
+      T_exists T2 (
+        T_equiv (app (lvar 1 term_var) (lvar 0 term_var)) (lvar 2 term_var)
+      )
+    )
+  ).
+
+Definition List : tree :=
+  intersect
+    (T_sum T_top T_top)
+    (T_sum T_unit (T_prod T_top (lvar 0 type_var))).
+
+Definition tnil := tleft uu.
+Definition Nil := tsingleton tnil.
+
+Definition tcons h t := tright (pp h t).
+Definition Cons H T :=
+  T_exists H (T_exists T (
+    tsingleton (tcons (lvar 1 term_var) (lvar 0 term_var))
+  )).
